Use the sink modality in the proof mode.
Whenever we iSpecialize something whose conclusion is persistent, we now have
to prove all the premises under the sink modality. This is strictly more powerful,
as we now have to use just some of the hypotheses to prove the premises, instead of
all.

theories/proofmode/classes.v
@@ -68,6 +68,12 @@ Arguments from_bare {_} _%I _%type_scope {_}.
 Hint Mode FromBare + ! - : typeclass_instances.
 Hint Mode FromBare + - ! : typeclass_instances.
 
+Class IntoSink {PROP : bi} (P Q : PROP) := into_sink : P ⊢ ▲ Q.
+Arguments IntoSink {_} _%I _%I.
+Arguments into_sink {_} _%I _%I {_}.
+Hint Mode IntoSink + ! -  : typeclass_instances.
+Hint Mode IntoSink + - ! : typeclass_instances.
+
 Class IntoInternalEq {PROP : bi} {A : ofeT} (P : PROP) (x y : A) :=
   into_internal_eq : P ⊢ x ≡ y.
 Arguments IntoInternalEq {_ _} _%I _%type_scope _%type_scope : simpl never.
